ulib/FStar.Seq.Base.fst
@@ -15,7 +15,7 @@
 *)
 
 (* A logical theory of sequences indexed by natural numbers in [0, n) *)
-module FStar.Seq
+module FStar.Seq.Base
 //#set-options "--initial_fuel 0 --max_fuel 0 --initial_ifuel 1 --max_ifuel 1"
 
 module List = FStar.List.Tot
