ulib/FStar.Seq.fst
@@ -1,0 +1,3 @@
+module FStar.Seq
+include FStar.Seq.Base
+include FStar.Seq.Properties
